src/Target_Definitions.v
@@ -4,6 +4,7 @@
 ***************************************************************************)
 
 Require Import Core_Definitions LibWfenv.
+Require Import ssreflect ssrbool ssrnat eqtype ssrfun seq path Eqdep.
 
 (* ********************************************************************** *)
 
@@ -17,11 +18,100 @@ Inductive t_type : typ -> Prop :=
   | t_type_pair : forall t1 t2,
       t_type t1 -> t_type t2 -> t_type (t_typ_pair t1 t2)
   | t_type_arrow : forall L t1 t2,
-      (forall X, X \notin L -> t_type (open_tt_var t1 X)) ->
-      (forall X, X \notin L -> t_type (open_tt_var t2 X)) ->
+      (forall X, X \notinLN L -> t_type (open_tt_var t1 X)) ->
+      (forall X, X \notinLN L -> t_type (open_tt_var t2 X)) ->
       t_type (t_typ_arrow t1 t2).
 
 Hint Constructors t_type.
+
+Fixpoint t_typeb (t : typ) : bool :=
+  match t with
+    t_typ_fvar x => true
+  | t_typ_bool  => true
+  | t_typ_pair t1 t2 => t_typeb t1 && t_typeb t2
+  | t_typ_arrow t1 t2 => t_typeb t1 && t_typeb t2
+  | _ => false
+  end.
+
+Lemma t_typeP : forall t : typ, reflect (t_type t) (t_typeb t). 
+Proof.
+move=> s.
+elim: s.
+by constructor; move=> tF; invert tF.
+by constructor; move=> tF; invert tF.
+move=> n.
+by constructor; move=> tF; invert tF.
+move=> v.
+by constructor; apply t_type_var.
+by constructor; apply t_type_bool.
+  move=> t1 t1P t2 t2P /=.
+  move: t1P t2P.
+  case: (t_typeb t1) => //=.
+  case: (t_typeb t2) => //=.
+  move=> t1P t2P.
+  case: t1P.
+  case: t2P.
+  move=> t2P t1P.
+  constructor.
+  apply t_type_pair; by [].
+  move=> t2P t1P.
+  constructor.
+  move=> tF.
+  apply t2P.
+  by invert tF.
+  move=> t1P.
+  constructor.
+  move=> tF.
+  apply t1P.
+  by invert tF.
+  move=> t1P t2P.
+  constructor.
+  move=> tF.
+  invert t2P => t2F.
+  apply t2F.
+  by invert tF.
+  move=> t1P t2P.
+  constructor.
+  move=> tF.
+  invert t1P => t2F.
+  apply t2F.
+  by invert tF.
+  move=> t1 t1P t2 t2P /=.
+  move: t1P t2P.
+  case: (t_typeb t1) => //=.
+  case: (t_typeb t2) => //=.
+  move=> t1P t2P.
+  case: t1P.
+  case: t2P.
+  move=> t2P t1P.
+  constructor.
+  apply t_type_arrow. by [].
+
+  move=> t2P t1P.
+  constructor.
+  move=> tF.
+  apply t2P.
+  by invert tF.
+  move=> t1P.
+  constructor.
+  move=> tF.
+  apply t1P.
+  by invert tF.
+  move=> t1P t2P.
+  constructor.
+  move=> tF.
+  invert t2P => t2F.
+  apply t2F.
+  by invert tF.
+  move=> t1P t2P.
+  constructor.
+  move=> tF.
+  invert t1P => t2F.
+  apply t2F.
+  by invert tF.
+
+
+
 
 (* Target Terms *)
 
@@ -31,11 +121,11 @@ Inductive t_term : trm -> Prop :=
       t_value u -> t_term m1 -> t_term m2 -> t_term (t_trm_if u m1 m2)
   | t_term_let_fst : forall L u m,
       t_value u ->
-      (forall x, x \notin L -> t_term (t_open_ee_var m x)) ->
+      (forall x, x \notinLN L -> t_term (t_open_ee_var m x)) ->
       t_term (t_trm_let_fst u m)
   | t_term_let_snd : forall L u m,
       t_value u ->
-      (forall x, x \notin L -> t_term (t_open_ee_var m x)) ->
+      (forall x, x \notinLN L -> t_term (t_open_ee_var m x)) ->
       t_term (t_trm_let_snd u m)
   | t_term_app : forall u1 t u2,
       t_value u1 -> t_type t -> t_value u2 -> t_term (t_trm_app u1 t u2)
@@ -47,8 +137,8 @@ with t_value : trm -> Prop :=
   | t_value_pair : forall u1 u2,
       t_value u1 -> t_value u2 -> t_value (t_trm_pair u1 u2)
   | t_value_abs  : forall L t m,
-      (forall X, X \notin L -> t_type (open_tt_var t X)) ->
-      (forall x X, x \notin L -> X \notin L ->
+      (forall X, X \notinLN L -> t_type (open_tt_var t X)) ->
+      (forall x X, x \notinLN L -> X \notinLN L ->
         t_term (open_te_var (t_open_ee_var m x) X)) ->
       t_value (t_trm_abs t m).
 
@@ -66,8 +156,8 @@ Inductive t_wft : env_type -> typ -> Prop :=
   | t_wft_pair : forall D t1 t2,
       t_wft D t1 -> t_wft D t2 -> t_wft D (t_typ_pair t1 t2)
   | t_wft_arrow : forall L D t1 t2,
-      (forall X, X \notin L -> t_wft (D & X ~ star) (open_tt_var t1 X)) ->
-      (forall X, X \notin L -> t_wft (D & X ~ star) (open_tt_var t2 X)) ->
+      (forall X, X \notinLN L -> t_wft (D & X ~ star) (open_tt_var t1 X)) ->
+      (forall X, X \notinLN L -> t_wft (D & X ~ star) (open_tt_var t2 X)) ->
       t_wft D (t_typ_arrow t1 t2).
 
 Hint Constructors t_wft.
@@ -83,11 +173,11 @@ Inductive t_typing : env_type -> env_term -> trm -> typ -> Prop :=
       t_typing D G (t_trm_if u m1 m2) t
   | t_typing_let_fst : forall L D G u m t1 t2 t,
       t_value_typing D G u (t_typ_pair t1 t2) ->
-      (forall x, x \notin L -> t_typing D (G & x ~ t1) (t_open_ee_var m x) t) ->
+      (forall x, x \notinLN L -> t_typing D (G & x ~ t1) (t_open_ee_var m x) t) ->
       t_typing D G (t_trm_let_fst u m) t
   | t_typing_let_snd : forall L D G u m t1 t2 t,
       t_value_typing D G u (t_typ_pair t1 t2) ->
-      (forall x, x \notin L -> t_typing D (G & x ~ t2) (t_open_ee_var m x) t) ->
+      (forall x, x \notinLN L -> t_typing D (G & x ~ t2) (t_open_ee_var m x) t) ->
       t_typing D G (t_trm_let_snd u m) t
   | t_typing_app : forall D G u1 u2 t t1 t2,
       t_value_typing D G u1 (t_typ_arrow t1 t2) ->
@@ -108,7 +198,7 @@ with t_value_typing : env_type -> env_term -> trm -> typ -> Prop :=
       t_value_typing D G (t_trm_pair u1 u2) (t_typ_pair t1 t2)
   | t_value_typing_abs : forall L D G m t1 t2,
       wfenv (t_wft D) G ->
-      (forall x X, x \notin L -> X \notin L ->
+      (forall x X, x \notinLN L -> X \notinLN L ->
         t_typing (D & X ~ star)
                  (G & x ~ (open_tt_var t1 X))
                  (open_te_var (t_open_ee_var m x) X)
@@ -140,19 +230,19 @@ Inductive t_context : bool (* accept only values? *) -> ctx -> Prop :=
       t_context b (t_ctx_if_false u m1 C)
   | t_context_let_fst : forall L b C m,
       t_value_context b C ->
-      (forall x, x \notin L -> t_term (t_open_ee_var m x)) ->
+      (forall x, x \notinLN L -> t_term (t_open_ee_var m x)) ->
       t_context b (t_ctx_let_fst C m)
   | t_context_let_fst_k : forall L u b C,
       t_value u ->
-      (forall x, x \notin L -> t_context b (t_ctx_open_ee_var C x)) ->
+      (forall x, x \notinLN L -> t_context b (t_ctx_open_ee_var C x)) ->
       t_context b (t_ctx_let_fst_k u C)
   | t_context_let_snd : forall L b C m,
       t_value_context b C ->
-      (forall x, x \notin L -> t_term (t_open_ee_var m x)) ->
+      (forall x, x \notinLN L -> t_term (t_open_ee_var m x)) ->
       t_context b (t_ctx_let_snd C m)
   | t_context_let_snd_k : forall L u b C,
       t_value u ->
-      (forall x, x \notin L -> t_context b (t_ctx_open_ee_var C x)) ->
+      (forall x, x \notinLN L -> t_context b (t_ctx_open_ee_var C x)) ->
       t_context b (t_ctx_let_snd_k u C)
   | t_context_app1 : forall b C t u,
       t_value_context b C -> t_type t -> t_value u ->
@@ -170,8 +260,8 @@ with t_value_context : bool (* accept only values? *) -> ctx -> Prop :=
       t_value u -> t_value_context b C ->
       t_value_context b (t_ctx_pair_right u C)
   | t_value_context_abs : forall L t b C,
-      (forall X, X \notin L -> t_type (open_tt_var t X)) ->
-      (forall x X, x \notin L -> X \notin L ->
+      (forall X, X \notinLN L -> t_type (open_tt_var t X)) ->
+      (forall x X, x \notinLN L -> X \notinLN L ->
         t_context b (ctx_open_te_var (t_ctx_open_ee_var C x) X)) ->
       t_value_context b (t_ctx_abs t C).
 
@@ -204,25 +294,25 @@ Inductive t_context_typing (* |- C : ( D ; G |- t ) ~> ( D' ; G' |- t' ) *)
       t_context_typing b (t_ctx_if_false u m1 C) D_hole G_hole t_hole D G t
   | t_context_typing_let_fst : forall b L Cv D_hole G_hole t_hole D G m t1 t2 t,
       t_value_context_typing b Cv D_hole G_hole t_hole D G (t_typ_pair t1 t2) ->
-      (forall x, x \notin L ->
+      (forall x, x \notinLN L ->
         t_typing D (G & x ~ t1) (t_open_ee_var m x) t) ->
       t_context_typing b (t_ctx_let_fst Cv m) D_hole G_hole t_hole D G t
   | t_context_typing_let_fst_k
     : forall b L C D_hole G_hole t_hole D G u t1 t2 t,
       t_value_typing D G u (t_typ_pair t1 t2) ->
-      (forall x, x \notin L ->
+      (forall x, x \notinLN L ->
         t_context_typing b (t_ctx_open_ee_var C x) D_hole G_hole t_hole
                                                    D (G & x ~ t1) t) ->
       t_context_typing b (t_ctx_let_fst_k u C) D_hole G_hole t_hole D G t
   | t_context_typing_let_snd : forall b L Cv D_hole G_hole t_hole D G m t1 t2 t,
       t_value_context_typing b Cv D_hole G_hole t_hole D G (t_typ_pair t1 t2) ->
-      (forall x, x \notin L ->
+      (forall x, x \notinLN L ->
         t_typing D (G & x ~ t2) (t_open_ee_var m x) t) ->
       t_context_typing b (t_ctx_let_snd Cv m) D_hole G_hole t_hole D G t
   | t_context_typing_let_snd_k
     : forall b L C D_hole G_hole t_hole D G u t1 t2 t,
       t_value_typing D G u (t_typ_pair t1 t2) ->
-      (forall x, x \notin L ->
+      (forall x, x \notinLN L ->
         t_context_typing b (t_ctx_open_ee_var C x) D_hole G_hole t_hole
                                                    D (G & x ~ t2) t) ->
       t_context_typing b (t_ctx_let_snd_k u C) D_hole G_hole t_hole D G t
@@ -262,7 +352,7 @@ with t_value_context_typing (* |- Cv : ( D ; G |- t ) ~> ( D' ; G' |- t' ) *)
                                                        D G (t_typ_pair t1 t2)
   | t_value_context_typing_abs : forall b L C D_hole G_hole t_hole D G t1 t2,
       wfenv (t_wft D) G ->
-      (forall x X, x \notin L -> X \notin L ->
+      (forall x X, x \notinLN L -> X \notinLN L ->
         t_context_typing b (ctx_open_te_var (t_ctx_open_ee_var C x) X)
                        D_hole G_hole t_hole
                        (D & X ~ star) (G & x ~ (open_tt_var t1 X))
