src/Backtranslation.v
@@ -15,8 +15,8 @@ Inductive subformula : env_term -> trm -> typ -> Prop :=
 | sf_s_false : forall G,
     wfenv trans_type G -> subformula G s_trm_false s_typ_bool
 | sf_s_abs : forall L G e s1 s2,
-    (forall x, x \notin L -> subformula (G & x ~ s1) (s_open_ee_var e x) s2) ->
-    (trans_type s1) ->
+    (forall x, x \notinLN L -> subformula (G & x ~ s1) (s_open_ee_var e x) s2) ->
+    (s_type s1) ->
     subformula G (s_trm_abs s1 e) (s_typ_arrow s1 s2)
 | sf_s_if : forall G e1 e2 e3 s,
     subformula G e1 s_typ_bool -> subformula G e2 s -> subformula G e3 s ->
@@ -34,13 +34,15 @@ Inductive subformula : env_term -> trm -> typ -> Prop :=
     wfenv trans_type G -> subformula G t_trm_false t_typ_bool
 | sf_t_abs : forall L G m s s1 s2,
     wfenv trans_type G ->
-    (forall x, x \notin L -> subformula (G & x ~ (s1+)) m (s2+)) ->
+    (* The follow may be wrong, we need to add the first projection of the functions argument to the context *)
+    (forall x, x \notinLN L ->
+      subformula (G & x ~ (t_typ_pair (s1+) (t_typ_arrow (s2+) (s2+)))) (t_open_ee_var m x) (s2+)) ->
     subformula G
     (* λ[α] (y,k) . let x = TS STe in (k x) *)
     (t_trm_abs (t_typ_pair (s1+) (t_typ_arrow (s2+) (t_typ_bvar 1)))
       (t_trm_ts (s_trm_st m s)
         s
-        (t_trm_let_snd (t_trm_bvar 0) (* let k = snd (x,k) in *)
+        (t_trm_let_snd (t_trm_bvar 1) (* let k = snd (y,k) in *)
         (t_trm_app (t_trm_bvar 0) (t_typ_bvar 0) (t_trm_bvar 1)))))
     ((s_typ_arrow s1 s2)+)
 | sf_t_if : forall G u m1 m2 t,
@@ -50,12 +52,73 @@ Inductive subformula : env_term -> trm -> typ -> Prop :=
 | sf_t_app : forall L G u1 u2a u2kontbody s s1 s2,
     subformula G u1 ((s_typ_arrow s1 s2)+) ->
     subformula G u2a (s1+) ->
-    (forall x, x \notin L -> subformula (G & x ~ (s2+)) (t_open_ee_var u2kontbody x) (s+)) ->
+    (forall x, x \notinLN L -> subformula (G & x ~ (s2+)) (t_open_ee_var u2kontbody x) (s+)) ->
     subformula G (t_trm_app u1 (s+) (t_trm_pair u2a (t_trm_abs (s2+) u2kontbody))) (s+)
 (* boundary type *)
 | sf_st : forall G m s,
     subformula G m (s+) -> subformula G (s_trm_st m s) s
 | sf_ts : forall L G e m s t,
     subformula G e s ->
-    (forall x, x \notin L -> subformula (G & x ~ (s+)) (t_open_ee_var m x) t) ->
+    (forall x, x \notinLN L -> subformula (G & x ~ (s+)) (t_open_ee_var m x) t) ->
     subformula G (t_trm_ts e s m) t.
+
+(* Partial reduction relation *)
+Inductive partial_eval : env_term -> trm -> typ -> trm -> Prop :=
+(* source type *)
+| sf_s_var : forall G x s,
+    wfenv trans_type G -> binds x s G -> partial_eval G (s_trm_fvar x) s (s_trm_fvar x)
+| sf_s_true : forall G,
+    wfenv trans_type G -> partial_eval G s_trm_true s_typ_bool s_trm_true
+| sf_s_false : forall G,
+    wfenv trans_type G -> partial_eval G s_trm_false s_typ_bool s_trm_false
+| sf_s_abs : forall L G e ep s1 s2,
+    (forall x, x \notinLN L -> partial_eval (G & x ~ s1) (s_open_ee_var e x) s2 (s_open_ee_var ep x)) ->
+    (s_type s1) ->
+    partial_eval G (s_trm_abs s1 e) (s_typ_arrow s1 s2) (s_trm_abs s1 ep)
+| sf_s_if : forall G e1 e1p e2 e2p e3 e3p s,
+    partial_eval G e1 s_typ_bool e1p -> partial_eval G e2 s e2p -> partial_eval G e3 s e3p ->
+    partial_eval G (s_trm_if e1 e2 e3) s (s_trm_if e1p e2p e3p)
+| sf_s_app : forall G e1 e1p e2 e2p s1 s2,
+    partial_eval G e1 (s_typ_arrow s1 s2) e1p -> partial_eval G e2 s1 e2p ->
+    partial_eval G (s_trm_app e1 e2) s2 (s_trm_app e1p e2p)
+(* trans type *)
+| sf_t_var : forall G x t,
+    wfenv trans_type G -> binds x t G ->
+    partial_eval G (t_trm_fvar x) t (t_trm_fvar x)
+| sf_t_true : forall G,
+    wfenv trans_type G -> partial_eval G t_trm_true t_typ_bool t_trm_true
+| sf_t_false : forall G,
+    wfenv trans_type G -> partial_eval G t_trm_false t_typ_bool t_trm_false
+| sf_t_abs : forall L G m mp s s1 s2,
+    wfenv trans_type G ->
+    (forall y, y \notinLN L -> partial_eval (G & y ~ (s1+))
+      (t_trm_let_fst (t_trm_bvar 0)
+        (t_open_ee (t_open_ee (open_te m (s2+)) t_id)) y))
+      (s2+) mp) ->
+    partial_eval G
+    (t_trm_abs (t_typ_pair (s1+) (t_typ_arrow (s2+) (t_typ_bvar 1)))
+      (t_trm_let_fst (t_trm_bvar 0)
+        (t_trm_let_snd (t_trm_bvar 1) m)))
+    ((s_typ_arrow s1 s2)+)
+    (* λ[α] (y,k) . let x = TS STe in (k x) *)
+    (t_trm_abs (t_typ_pair (s1+) (t_typ_arrow (s2+) (t_typ_bvar 1)))
+      (t_trm_ts (s_trm_st mp s)
+        s
+        (t_trm_let_snd (t_trm_bvar 0) (* let k = snd (x,k) in *)
+        (t_trm_app (t_trm_bvar 0) (t_typ_bvar 0) (t_trm_bvar 1)))))
+| sf_t_if : forall G u up m1 m1p m2 m2p t,
+    partial_eval G u t_typ_bool up ->
+    partial_eval G m1 t m1p -> partial_eval G m2 t m2p ->
+    partial_eval G (t_trm_if u m1 m2) t (t_trm_if up m1p m2p)
+| sf_t_app : forall L G u1 u1p u2a u2ap u2kontbody u2kontbodyp s s1 s2,
+    partial_eval G u1 ((s_typ_arrow s1 s2)+) u1p ->
+    partial_eval G u2a (s1+) u2ap ->
+    (forall x, x \notinLN L -> partial_eval (G & x ~ (s2+)) (t_open_ee_var u2kontbody x) (s+)) (t_open_ee_var u2kontbodyp x)->
+    partial_eval G (t_trm_app u1 (s+) (t_trm_pair u2a (t_trm_abs (s2+) u2kontbody))) (s+)
+(* boundary type *)
+| sf_st : forall G m mp s,
+    partial_eval G m (s+) mp -> partial_eval G (s_trm_st m s) s (s_trm_st mp s)
+| sf_ts : forall L G e ep m mp s t,
+    partial_eval G e s ep ->
+    (forall x, x \notinLN L -> partial_eval (G & x ~ (s+)) (t_open_ee_var m x) t (t_open_ee_var mp x)) ->
+    partial_eval G (t_trm_ts e s m) t (t_trm_ts ep s mp).
