src/Target_Properties.v
@@ -47,14 +47,14 @@ Qed.
 (* t_wft and free variables *)
 
 Lemma t_wft_fv_tt : forall t D X,
-  t_wft D t -> X \in fv_tt t -> X \in dom D.
+  t_wft D t -> X \inLN fv_tt t -> X \inLN dom D.
 Proof.
   intros D t X wft. gen X.
   induction wft; simpl; intros; auto.
   rewrite in_singleton in H1. subst. apply* get_some_inv.
   false. apply* in_empty_elim.
   rewrite in_union in H. intuition.
-  pick_fresh Y. assert (X \in dom (D & Y ~ star)).
+  pick_fresh Y. assert (X \inLN dom (D & Y ~ star)).
     rewrite in_union in H3. destruct H3.
     assert (fv_tt (open_tt_var t1 Y) = fv_tt t1 \u \{Y} \/ fv_tt (open_tt_var t1 Y) = fv_tt t1).
       apply open_tt_var_fv_tt.
@@ -68,7 +68,7 @@ Proof.
 Qed.
 
 Lemma t_wft_fv_tt_inv : forall t D X,
-  t_wft D t -> X \notin dom D -> X \notin fv_tt t.
+  t_wft D t -> X \notinLN dom D -> X \notinLN fv_tt t.
 Proof.
   intros. intro. apply (t_wft_fv_tt t D) in H1; intuition.
 Qed.
@@ -125,7 +125,7 @@ Proof.
 Qed.
 
 Lemma subst_tt_intro_rec : forall X t t' n,
-  X \notin fv_tt t -> t_type t' ->
+  X \notinLN fv_tt t -> t_type t' ->
   open_tt_rec n t' t = subst_tt (X ~ t') (open_tt_rec n (t_typ_fvar X) t).
 Proof.
   intros X t. gen X. induction t; intros; auto; simpl in *; try f_equal; auto.
@@ -134,7 +134,7 @@ Proof.
 Qed.
 
 Lemma subst_tt_intro : forall X t t',
-  X \notin fv_tt t -> t_type t' ->
+  X \notinLN fv_tt t -> t_type t' ->
   open_tt t t' = subst_tt (X ~ t') (open_tt_var t X).
 Proof.
   intros. apply* subst_tt_intro_rec.
